`conv start`

`example_user`
Goals to prove:
x y : ℝ
h1: x = 3 - 2 * y
h2: 2 * (3 - 2 * y) - y = 1
⊢ y = 1

[STEPS]
rw [h1] at h2

[INCORRECT STEPS]
[❌] rw [h2] at h1

[LAST STEP]
rw [h2] at h1

[ERROR MESSAGE]
tactic 'rewrite' failed, did not find instance of the pattern in the target expression
  2 * (3 - 2 * y) - y
state: 
x y : ℝ
h1 : x = 3 - 2 * y
h2 : 2 * (3 - 2 * y) - y = 1
⊢ y = 1
[END]

`example_assistant`
[RUN TACTIC]
linarith
[END]

`example_user`
Goals to prove:
n : ℕ
h0 : n < 398 
h1 : (n * 7) % 398 = 1
⊢ n = 57

[LAST STEP]
norm_num
[ERROR MESSAGE]
unsolved goals
state:
n : ℕ
h0 : n < 398
h1 : n * 7 % 398 = 1
⊢ n = 57
[END]

`example_assistant`
[RUN TACTIC]
-- We can create an intermediate lemma to help prove the goal
-- First actually prove that (57 * 7) % 398 = 1, then use that to show n = 57
-- let's start by adding the new lemma
have h2 : 1 % 398 = (57 * 7) % 398 := by
[END]

`example_user`
Goals to prove:
a b : Nat
h0 : a < 3
h1 : b < a
h3 : 1 < b
⊢ b = 2

[END]

`example_assistant`
[RUN TACTIC]
-- Since there are finite many cases, we can just use grind
grind
[END]

`example_user`
Goals to prove:
(s : ℕ → ℝ)
h0: ∀ n, s (n + 2) = s (n + 1) + s n
h1 : s 9 = 110
h2 : s 7 = 42
h : ∀ (n : ℕ), s n = s (n + 2) - s (n + 1)
h3 : s 9 = s 8 + s 7
h4 : s 8 = 68
⊢ s 5 = 16

[STEPS]
have h : ∀ n, s n = s (n + 2) - s (n + 1) := by 
  intro n; 
  simp [h0 n]
have h3 : s 9 = s 8 + s 7 := h0 7
have h4 : s 8 = 68 := by 
  linarith


[LAST STEP]
linarith
[ERROR MESSAGE]
linarith failed to find a contradiction
state:
s : ℕ → ℕ
h₀ : ∀ (n : ℕ), s (n + 2) = s (n + 1) + s n
h₁ : s 9 = 110
h₂ : s 7 = 42
h : ∀ (n : ℕ), s n = s (n + 2) - s (n + 1)
h₃ : s 9 = s 8 + s 7
h₄ : s 8 = 68
a✝ : s 5 < 16
⊢ false
[END]

`example_assistant`
[RUN TACTIC]
rw [(h 5)]
[END]

`example_user`
Goals to prove:
p q : Prop
hp : p
hq : q
⊢ p ∧ q ∧ p

[END]

`example_assistant`
[RUN TACTIC]
-- We can start by defining a simple lemma
-- proving p ∧ q and then simplify the existing goal
-- to prove the whole thing in one go.
have hpq : p ∧ q := by
  apply And.intro
  exact hp
  assumption
-- finally, we can use simp to finish the proof
simp [hpq]
[END]

`example_user`
Goals to prove:
d : ℕ
id : 3 ∣ d ^ 3 + 2 * d
id_expanded : (d + 1) ^ 3 + 2 * (d + 1) = d ^ 3 + 3 * d ^ 2 + 5 * d + 3
id_factored : d ^ 3 + 3 * d ^ 2 + 5 * d + 3 = d ^ 3 + 2 * d + 3 * (d ^ 2 + d + 1)
⊢ 3 ∣ d ^ 3 + 2 * d + 3 * (d ^ 2 + d + 1)

[STEPS]
induction' n with d ih
simp
have ih_expanded : (d + 1)^3 + 2 * (d + 1) = d^3 + 3 * d^2 + 5 * d + 3 := by 
  ring
rw [ih_expanded]
have ih_factored : d^3 + 3 * d^2 + 5 * d + 3 = d^3 + 2 * d + 3 * (d^2 + d + 1) := by 
  ring

[LAST STEP]
rw [ih_factored]
[SUCCESS]
[END]

`example_assistant`
[RUN TACTIC]
    apply dvd_add ih
[END]

`example_user`
Goals to prove:
b : ℝ
f : ℝ → ℝ
h₀ : ∀ (x : ℝ), f x = 3 * x ^ 4 - 7 * x ^ 3 + 2 * x ^ 2 - b * x + 1
h₁ : 3 * 1 ^ 4 - 7 * 1 ^ 3 + 2 * 1 ^ 2 - b * 1 + 1 = 1
⊢ b = -2

[LAST STEP]
rw h₀ at h₁
[SUCCESS]
[END]

`example_assistant`
[RUN TACTIC]
norm_num at h1
[END]


`conv end`